proofmode/weakestpre.v
@@ -8,10 +8,15 @@ Context {Λ : language} {Σ : iFunctor}.
 Implicit Types P Q : iProp Λ Σ.
 Implicit Types Φ : val Λ → iProp Λ Σ.
 
-Global Instance frame_wp E e R Φ Ψ :
-  (∀ v, Frame R (Φ v) (Ψ v)) → Frame R (WP e @ E {{ Φ }}) (WP e @ E {{ Ψ }}).
+Instance frame_wp E e R Φ mΨ :
+  (∀ v, Frame R (Φ v) (mΨ v)) →
+  Frame R (WP e @ E {{ Φ }})
+          (Some (WP e @ E {{ v, if mΨ v is Some Q then Q else True }}))%I.
 Proof. rewrite /Frame=> HR. rewrite wp_frame_l. apply wp_mono, HR. Qed.
 Global Instance fsa_split_wp E e Φ :
   FSASplit (WP e @ E {{ Φ }})%I E (wp_fsa e) (language.atomic e) Φ.
 Proof. split. done. apply _. Qed.
 End weakestpre.
+
+Hint Extern 10 (Frame _ (WP _ @ _ {{ _ }}) _) =>
+  class_apply frame_wp : typeclass_instances.
